tests/lean/run/idSuggestEvery.lean
@@ -1,0 +1,102 @@
+-- test every/all replacements in default imports
+
+example := (·.all)
+example := (·.contains)
+example := (Array.contains)
+
+/-
+Expected replacements for `Subarray.any` and `Subarray.all` do not work as suggestion annotations
+when using generalized field notation: Subarray is an abbreviation and so the underlying `Std.Slice`
+type, which does not have a corresponding `.any`/`.all` function.
+-/
+
+/--
+error: Invalid field `every`: The environment does not contain `Std.Slice.every`, so it is not possible to project the field `every` from an expression
+  x
+of type
+  Std.Slice (Std.Slice.Internal.SubarrayData Nat)
+-/
+#guard_msgs in example (x : Subarray Nat) := x.every fun _ => true
+#guard_msgs in example (x : Subarray Nat) := x.all fun _ => true
+
+/--
+error: Unknown constant `Subarray.every`
+
+Hint: Perhaps you meant `Subarray.all` in place of `Subarray.every`:
+  S̵u̵b̵a̵r̵r̵a̵y̵.̵e̵v̵e̵r̵y̵S̲u̲b̲a̲r̲r̲a̲y̲.̲a̲l̲l̲
+-/
+#guard_msgs in example := (@Subarray.every Nat (fun _ => true) ·)
+#guard_msgs in example := (@Subarray.all Nat (fun _ => true) ·)
+
+/--
+error: Unknown constant `Subarray.some`
+
+Hint: Perhaps you meant `Subarray.any` in place of `Subarray.some`:
+  S̵u̵b̵a̵r̵r̵a̵y̵.̵s̵o̵m̵e̵S̲u̲b̲a̲r̲r̲a̲y̲.̲a̲n̲y̲
+-/
+#guard_msgs in example := (@Subarray.some Nat (fun _ => true) ·)
+#guard_msgs in example := (@Subarray.any Nat (fun _ => true) ·)
+
+/--
+error: Invalid field `every`: The environment does not contain `String.every`, so it is not possible to project the field `every` from an expression
+  x
+of type `String`
+
+Hint: Perhaps you meant `String.all` in place of `String.every`:
+  .e̵v̵e̵r̵y̵a̲l̲l̲
+-/
+#guard_msgs in example (x : String) := x.every fun _ => true
+#guard_msgs in example (x : String) := x.all fun _ => true
+/--
+error: Invalid field `some`: The environment does not contain `String.some`, so it is not possible to project the field `some` from an expression
+  x
+of type `String`
+
+Hint: Perhaps you meant `String.contains` in place of `String.some`:
+  .s̵o̵m̵e̵c̲o̲n̲t̲a̲i̲n̲s̲
+-/
+#guard_msgs in example (x : String) := x.some fun _ => true
+#guard_msgs in example (x : String) := x.all fun _ => true
+
+
+/--
+error: Invalid field `every`: The environment does not contain `Array.every`, so it is not possible to project the field `every` from an expression
+  x
+of type `Array Nat`
+
+Hint: Perhaps you meant `Array.all` in place of `Array.every`:
+  .e̵v̵e̵r̵y̵a̲l̲l̲
+-/
+#guard_msgs in example (x : Array Nat) := x.every fun _ => true
+#guard_msgs in example (x : Array Nat) := x.all fun _ => true
+/--
+error: Invalid field `some`: The environment does not contain `Array.some`, so it is not possible to project the field `some` from an expression
+  x
+of type `Array Nat`
+
+Hint: Perhaps you meant `Array.any` in place of `Array.some`:
+  .s̵o̵m̵e̵a̲n̲y̲
+-/
+#guard_msgs in example (x : Array Nat) := x.some fun _ => true
+#guard_msgs in example (x : Array Nat) := x.all fun _ => true
+
+/--
+error: Invalid field `every`: The environment does not contain `List.every`, so it is not possible to project the field `every` from an expression
+  x
+of type `List Nat`
+
+Hint: Perhaps you meant `List.all` in place of `List.every`:
+  .e̵v̵e̵r̵y̵a̲l̲l̲
+-/
+#guard_msgs in example (x : List Nat) := x.every fun _ => true
+#guard_msgs in example (x : List Nat) := x.all fun _ => true
+/--
+error: Invalid field `some`: The environment does not contain `List.some`, so it is not possible to project the field `some` from an expression
+  x
+of type `List Nat`
+
+Hint: Perhaps you meant `List.any` in place of `List.some`:
+  .s̵o̵m̵e̵a̲n̲y̲
+-/
+#guard_msgs in example (x : List Nat) := x.some fun _ => true
+#guard_msgs in example (x : List Nat) := x.all fun _ => true
